Add requirement that computable equality is well typed

ComputableEquality.v
@@ -1,13 +1,19 @@
 Require Import List.
 Import ListNotations.
 
-Require Export SystemFR.ReducibilityLemmas.
+Require Export SystemFR.ErasedArrow.
+Require Export SystemFR.ErasedBool.
+Require Export SystemFR.ErasedPair.
 Require Export SystemFR.NatEq.
 Require Export SystemFR.EquivalenceLemmas2.
 
 Opaque reducible_values.
 
 Definition computable_equality_with f_eq theta T : Prop :=
+  wf f_eq 0 /\
+  is_erased_term f_eq /\
+  pfv f_eq term_var = nil /\
+  reducible theta f_eq (T_arrow T (T_arrow T T_bool)) /\
   forall v1 v2,
     reducible_values theta v1 T ->
     reducible_values theta v2 T ->
@@ -16,20 +22,31 @@ Definition computable_equality_with f_eq theta T : Prop :=
 
 Definition computable_equality theta T : Prop :=
   exists f_eq,
-    wf f_eq 0 /\
-    is_erased_term f_eq /\
-    pfv f_eq term_var = nil /\
     computable_equality_with f_eq theta T.
 
 Lemma computable_equality_subtype:
   forall theta A B,
     computable_equality theta A ->
+    valid_interpretation theta ->
     subtype theta B A ->
+    is_erased_type B ->
+    wf A 0 ->
+    wf B 0 ->
     computable_equality theta B.
 Proof.
   unfold computable_equality, computable_equality_with;
-    repeat step;
-    eauto with apply_any step_tactic.
+    repeat step.
+
+  eexists; steps;
+    eauto with apply_any.
+
+  eapply reducible_values_exprs; try eassumption;
+    repeat step || simp_red || apply_any || open_none.
+
+  repeat unfold reduces_to in *; steps; t_closer.
+
+  unshelve epose proof (H18 a _ _ _ _); repeat step || open_none.
+  exists v; repeat step || simp_red.
 Qed.
 
 Lemma computable_equality_prod:
@@ -37,6 +54,10 @@ Lemma computable_equality_prod:
     valid_interpretation theta ->
     wf A 0 ->
     wf B 0 ->
+    is_erased_type A ->
+    is_erased_type B ->
+    pfv A term_var = nil ->
+    pfv B term_var = nil ->
     computable_equality theta A ->
     computable_equality theta B ->
     computable_equality theta (T_prod A B).
@@ -48,19 +69,31 @@ Proof.
         tfalse)));
     repeat step || simp_red || list_utils; eauto with wf.
 
+  - apply reducible_value_expr; auto.
+    apply reducible_lambda; repeat step || list_utils || open_none; t_closer.
+    apply reducible_value_expr; auto.
+    apply reducible_lambda; repeat step || list_utils || open_none; t_closer.
+
+    apply reducible_ite; repeat step; t_closer;
+      eauto using reducible_value_expr, reducible_false.
+    + apply reducible_app2 with A; steps; eauto using reducible_value_expr, reducible_pi1.
+      apply reducible_app2 with A; steps; eauto using reducible_value_expr, reducible_pi1.
+    + apply reducible_app2 with B; steps; eauto using reducible_value_expr, reducible_pi2_nodep.
+      apply reducible_app2 with B; steps; eauto using reducible_value_expr, reducible_pi2_nodep.
+
   - reverse_once; repeat open_none; eauto with values.
     reverse_once; repeat open_none.
     reverse_once; repeat open_none || step; eauto with values.
-    apply star_smallstep_value in H39; steps; eauto with values.
-    apply star_smallstep_value in H40; steps; eauto with values.
+    apply star_smallstep_value in H45; steps; eauto with values.
+    apply star_smallstep_value in H46; steps; eauto with values.
     reverse_once; repeat open_none.
     apply equivalent_pp.
-    + apply H10; steps.
+    + apply H16; steps.
       apply equivalent_star_true with (app (app f_eq0 (pi1 (pp a0 b0))) (pi1 (pp v1 v0)));
         repeat apply equivalent_app || step;
         try solve [ apply equivalent_refl; steps ];
         try solve [ apply equivalent_star; steps; t_closer; eauto using star_one with smallstep ].
-    + apply H7; steps.
+    + apply H12; steps.
       apply equivalent_star_true with (app (app f_eq (pi2 (pp a0 b0))) (pi2 (pp v1 v0)));
         repeat apply equivalent_app || step;
         try solve [ apply equivalent_refl; steps ];
@@ -84,12 +117,42 @@ Proof.
         eauto with apply_any.
 Qed.
 
-Lemma computable_equality_nat:
+Lemma computable_equality_with_nat_eq:
   computable_equality_with nat_eq_fix [] T_nat.
 Proof.
-  unfold computable_equality_with; repeat step || simp_red.
+  unfold computable_equality_with; repeat step || simp_red; eauto with lia.
+  - unfold nat_eq_fix.
+    eapply backstep_reducible; steps; eauto with lia; eauto with smallstep;
+      repeat step.
+
+    apply reducible_value_expr; steps.
+    apply reducible_lambda; steps; eauto with lia.
+    apply reducible_value_expr; steps.
+    assert (valid_interpretation []); steps.
+    apply reducible_lambda; repeat step || simp_red || list_utils || open_none; eauto with lia; t_closer.
+
+    apply star_smallstep_reducible with (nat_eq u u0);
+      repeat step || unfold reducible, reduces_to;
+      try solve [
+        unfold nat_eq, nat_eq_fix, closed_term; repeat step || list_utils; eauto with lia; t_closer
+      ].
+
+    + unfold nat_eq, nat_eq_fix.
+      one_step; steps.
+      one_step; steps.
+      one_step; steps.
+    + unshelve epose proof (nat_eq_bool u _ u0 _); steps;
+        try solve [ eexists; steps; try eassumption; repeat step || simp_red ].
+
   - apply_anywhere nat_eq_sound; steps; t_closer.
     apply equivalent_refl; t_closer.
   - apply_anywhere equivalent_value_nat; steps; eauto with values;
       eauto using nat_eq_complete2.
+Qed.
+
+Lemma computable_equality_nat:
+  computable_equality [] T_nat.
+Proof.
+  unfold computable_equality;
+    eauto using computable_equality_with_nat_eq.
 Qed.
